tests/vfmTestHelperScript.sml
@@ -26,12 +26,8 @@ End
 
 (* TODO: move to another theory? *)
 
-Definition block_header_from_block_rlp_def:
-  block_header_from_block_rlp rlp =
-  if ¬is_RLPL rlp then NONE else
-  let ls = dest_RLPL rlp in
-  if LENGTH ls ≠ 4 then NONE else
-  let rlp = EL 0 ls in
+Definition block_header_from_rlp_def:
+  block_header_from_rlp rlp =
   if ¬is_RLPL rlp then NONE else
   let ls = dest_RLPL rlp in
   if ¬(LENGTH ls = 20 ∧ EVERY is_RLPB ls) then NONE else
@@ -87,23 +83,418 @@ Definition block_header_from_block_rlp_def:
      |>
 End
 
-val block_header_from_block_rlp_pre_def =
-  cv_auto_trans_pre block_header_from_block_rlp_def;
+val block_header_from_rlp_pre_def =
+  cv_auto_trans_pre block_header_from_rlp_def;
 
-Theorem block_header_from_block_rlp_pre[cv_pre]:
-  block_header_from_block_rlp_pre x
+Theorem block_header_from_rlp_pre[cv_pre]:
+  block_header_from_rlp_pre x
 Proof
-  rw[block_header_from_block_rlp_pre_def]
+  rw[block_header_from_rlp_pre_def]
   \\ Cases_on`x` \\ gvs[]
   \\ strip_tac \\ gvs[]
 QED
 
+Definition withdrawal_from_rlp_def:
+  withdrawal_from_rlp rlp =
+  if ¬is_RLPL rlp then NONE else
+  let ls = dest_RLPL rlp in
+  if ¬(LENGTH ls = 4 ∧ EVERY is_RLPB ls) then NONE else
+  let index = EL 0 ls in
+  let validatorIndex = EL 1 ls in
+  let address = EL 2 ls in
+  let amount = EL 3 ls in
+  SOME <|
+    withdrawalIndex := num_of_be_bytes (dest_RLPB index)
+  ; validatorIndex := num_of_be_bytes (dest_RLPB validatorIndex)
+  ; withdrawalAddress := word_of_bytes T 0w (dest_RLPB address)
+  ; withdrawalAmount := num_of_be_bytes (dest_RLPB amount)
+  |>
+End
+
+val withdrawal_from_rlp_pre_def = cv_auto_trans_pre withdrawal_from_rlp_def;
+
+Theorem withdrawal_from_rlp_pre[cv_pre]:
+  withdrawal_from_rlp_pre x
+Proof
+  rw[withdrawal_from_rlp_pre_def]
+  \\ strip_tac \\ gvs[]
+QED
+
+Definition access_list_entry_from_rlp_def:
+  access_list_entry_from_rlp rlp =
+  if ¬is_RLPL rlp then NONE else
+  let ls = dest_RLPL rlp in
+  if LENGTH ls ≠ 2 then NONE else
+  let account = EL 0 ls in
+  if ¬is_RLPB account then NONE else
+  let account = word_of_bytes T 0w $ dest_RLPB account in
+  let slots = EL 1 ls in
+  if ¬is_RLPL slots then NONE else
+  let ls = dest_RLPL slots in
+  if ¬(EVERY is_RLPB ls) then NONE else
+  let slots = MAP (word_of_bytes T 0w o dest_RLPB) ls in
+  SOME <| account := account; keys := slots |>
+End
+
+val access_list_entry_from_rlp_pre_def =
+  cv_auto_trans_pre access_list_entry_from_rlp_def;
+
+Theorem access_list_entry_from_rlp_pre[cv_pre]:
+  access_list_entry_from_rlp_pre x
+Proof
+  rw[access_list_entry_from_rlp_pre_def]
+  \\ strip_tac \\ gvs[]
+QED
+
+Definition OPT_MMAP_access_list_entry_from_rlp_def:
+  OPT_MMAP_access_list_entry_from_rlp [] = SOME [] ∧
+  OPT_MMAP_access_list_entry_from_rlp (x::xs) =
+  case access_list_entry_from_rlp x of NONE => NONE
+     | SOME h =>
+         case OPT_MMAP_access_list_entry_from_rlp xs of NONE => NONE
+            | SOME t => SOME (h::t)
+End
+
+val () = cv_auto_trans OPT_MMAP_access_list_entry_from_rlp_def;
+
+Theorem OPT_MMAP_access_list_entry_from_rlp_eq:
+  OPT_MMAP_access_list_entry_from_rlp ls =
+  OPT_MMAP access_list_entry_from_rlp ls
+Proof
+  Induct_on`ls` \\ rw[OPT_MMAP_access_list_entry_from_rlp_def]
+  \\ CASE_TAC \\ gvs[]
+  \\ CASE_TAC \\ gvs[]
+QED
+
+Definition transaction1_from_rlp_def:
+  transaction1_from_rlp rlp =
+  if ¬is_RLPL rlp then NONE else
+  let ls = dest_RLPL rlp in
+  if LENGTH ls ≠ 11 then NONE else
+  (* chain_id: U64 *)
+  let nonce = EL 1 ls in
+  if ¬is_RLPB nonce then NONE else
+  let nonce = num_of_be_bytes $ dest_RLPB nonce in
+  let gasPrice = EL 2 ls in
+  if ¬is_RLPB gasPrice then NONE else
+  let gasPrice = num_of_be_bytes $ dest_RLPB gasPrice in
+  let gas = EL 3 ls in
+  if ¬is_RLPB gas then NONE else
+  let gas = num_of_be_bytes $ dest_RLPB gas in
+  let to = EL 4 ls in
+  if ¬is_RLPB to then NONE else
+  let to = dest_RLPB to in
+  let to = if LENGTH to = 0 then NONE
+           else SOME $ word_of_bytes T 0w to in
+  let value = EL 5 ls in
+  if ¬is_RLPB value then NONE else
+  let value = num_of_be_bytes $ dest_RLPB value in
+  let data = EL 6 ls in
+  if ¬is_RLPB data then NONE else
+  let data = dest_RLPB data in
+  let accessList = EL 7 ls in
+  if ¬is_RLPL accessList then NONE else
+  case OPT_MMAP access_list_entry_from_rlp (dest_RLPL accessList)
+  of NONE => NONE |
+  SOME accessList =>
+  let yParity = EL 8 ls in
+  let r = EL 9 ls in
+  let s = EL 10 ls in
+  SOME <|
+      from := 0w (* TODO: ecrecover from yParity r s *)
+    ; to := to
+    ; data := data
+    ; nonce := nonce
+    ; value := value
+    ; gasLimit := gas
+    ; gasPrice := gasPrice
+    ; accessList := accessList
+    ; blobVersionedHashes := []
+    ; maxFeePerBlobGas := NONE
+    ; maxFeePerGas := NONE
+  |>
+End
+
+val transaction1_from_rlp_pre_def = transaction1_from_rlp_def
+  |> SRULE [GSYM OPT_MMAP_access_list_entry_from_rlp_eq]
+  |> cv_auto_trans_pre;
+
+Theorem transaction1_from_rlp_pre[cv_pre]:
+  transaction1_from_rlp_pre x
+Proof
+  rw[transaction1_from_rlp_pre_def]
+QED
+
+Definition transaction2_from_rlp_def:
+  transaction2_from_rlp baseFee rlp =
+  if ¬is_RLPL rlp then NONE else
+  let ls = dest_RLPL rlp in
+  if LENGTH ls ≠ 12 then NONE else
+  (* chain_id: U64 *)
+  let nonce = EL 1 ls in
+  if ¬is_RLPB nonce then NONE else
+  let nonce = num_of_be_bytes $ dest_RLPB nonce in
+  let maxPrio = EL 2 ls in
+  if ¬is_RLPB maxPrio then NONE else
+  let maxPrio = num_of_be_bytes $ dest_RLPB maxPrio in
+  let maxFee = EL 3 ls in
+  if ¬is_RLPB maxFee then NONE else
+  let maxFee = num_of_be_bytes $ dest_RLPB maxFee in
+  let gas = EL 4 ls in
+  if ¬is_RLPB gas then NONE else
+  let gas = num_of_be_bytes $ dest_RLPB gas in
+  let to = EL 5 ls in
+  if ¬is_RLPB to then NONE else
+  let to = dest_RLPB to in
+  let to = if LENGTH to = 0 then NONE
+           else SOME $ word_of_bytes T 0w to in
+  let value = EL 6 ls in
+  if ¬is_RLPB value then NONE else
+  let value = num_of_be_bytes $ dest_RLPB value in
+  let data = EL 7 ls in
+  if ¬is_RLPB data then NONE else
+  let data = dest_RLPB data in
+  let accessList = EL 8 ls in
+  if ¬is_RLPL accessList then NONE else
+  case OPT_MMAP access_list_entry_from_rlp (dest_RLPL accessList)
+  of NONE => NONE |
+  SOME accessList =>
+  let yParity = EL 9 ls in
+  let r = EL 10 ls in
+  let s = EL 11 ls in
+  SOME <|
+      from := 0w (* TODO: ecrecover from yParity r s *)
+    ; to := to
+    ; data := data
+    ; nonce := nonce
+    ; value := value
+    ; gasLimit := gas
+    ; gasPrice := effective_gas_price baseFee maxFee maxPrio
+    ; accessList := accessList
+    ; blobVersionedHashes := []
+    ; maxFeePerBlobGas := NONE
+    ; maxFeePerGas := SOME maxFee
+  |>
+End
+
+val transaction2_from_rlp_pre_def = transaction2_from_rlp_def
+  |> SRULE [GSYM OPT_MMAP_access_list_entry_from_rlp_eq]
+  |> cv_auto_trans_pre;
+
+Theorem transaction2_from_rlp_pre[cv_pre]:
+  transaction2_from_rlp_pre bf x
+Proof
+  rw[transaction2_from_rlp_pre_def]
+QED
+
+Definition transaction3_from_rlp_def:
+  transaction3_from_rlp baseFee rlp =
+  if ¬is_RLPL rlp then NONE else
+  let ls = dest_RLPL rlp in
+  if LENGTH ls ≠ 14 then NONE else
+  (* chain_id: U64 *)
+  let nonce = EL 1 ls in
+  if ¬is_RLPB nonce then NONE else
+  let nonce = num_of_be_bytes $ dest_RLPB nonce in
+  let maxPrio = EL 2 ls in
+  if ¬is_RLPB maxPrio then NONE else
+  let maxPrio = num_of_be_bytes $ dest_RLPB maxPrio in
+  let maxFee = EL 3 ls in
+  if ¬is_RLPB maxFee then NONE else
+  let maxFee = num_of_be_bytes $ dest_RLPB maxFee in
+  let gas = EL 4 ls in
+  if ¬is_RLPB gas then NONE else
+  let gas = num_of_be_bytes $ dest_RLPB gas in
+  let to = EL 5 ls in
+  if ¬is_RLPB to then NONE else
+  let to = dest_RLPB to in
+  let to = if LENGTH to = 0 then NONE
+           else SOME $ word_of_bytes T 0w to in
+  let value = EL 6 ls in
+  if ¬is_RLPB value then NONE else
+  let value = num_of_be_bytes $ dest_RLPB value in
+  let data = EL 7 ls in
+  if ¬is_RLPB data then NONE else
+  let data = dest_RLPB data in
+  let accessList = EL 8 ls in
+  if ¬is_RLPL accessList then NONE else
+  case OPT_MMAP access_list_entry_from_rlp (dest_RLPL accessList)
+  of NONE => NONE |
+  SOME accessList =>
+  let maxBlobFee = EL 9 ls in
+  if ¬is_RLPB maxBlobFee then NONE else
+  let maxBlobFee = num_of_be_bytes $ dest_RLPB maxBlobFee in
+  let blobHashes = EL 10 ls in
+  if ¬is_RLPL blobHashes then NONE else
+  let blobHashes = dest_RLPL blobHashes in
+  if ¬(EVERY is_RLPB blobHashes) then NONE else
+  let blobHashes = MAP (word_of_bytes T 0w o dest_RLPB) blobHashes in
+  let yParity = EL 11 ls in
+  let r = EL 12 ls in
+  let s = EL 13 ls in
+  SOME <|
+      from := 0w (* TODO: ecrecover from yParity r s *)
+    ; to := to
+    ; data := data
+    ; nonce := nonce
+    ; value := value
+    ; gasLimit := gas
+    ; gasPrice := effective_gas_price baseFee maxFee maxPrio
+    ; accessList := accessList
+    ; blobVersionedHashes := blobHashes
+    ; maxFeePerBlobGas := SOME maxBlobFee
+    ; maxFeePerGas := SOME maxFee
+  |>
+End
+
+val transaction3_from_rlp_pre_def = transaction3_from_rlp_def
+  |> SRULE [GSYM OPT_MMAP_access_list_entry_from_rlp_eq]
+  |> cv_auto_trans_pre;
+
+Theorem transaction3_from_rlp_pre[cv_pre]:
+  transaction3_from_rlp_pre bf x
+Proof
+  rw[transaction3_from_rlp_pre_def]
+QED
+
+Definition transaction_from_rlp_def:
+  transaction_from_rlp baseFee rlp =
+  if is_RLPL rlp then
+    let ls = dest_RLPL rlp in
+    if ¬(LENGTH ls = 9 ∧ EVERY is_RLPB ls) then NONE else
+    let nonce = EL 0 ls in
+    let gasPrice = EL 1 ls in
+    let gas = EL 2 ls in
+    let to = dest_RLPB $ EL 3 ls in
+    let value = EL 4 ls in
+    let data = EL 5 ls in
+    let v = EL 6 ls in
+    let r = EL 7 ls in
+    let s = EL 8 ls in
+      SOME <|
+        from := 0w (* TODO: ecrecover from v r s *)
+      ; to := if LENGTH to = 0 then NONE
+              else SOME $ word_of_bytes T 0w to
+      ; data := dest_RLPB data
+      ; nonce := num_of_be_bytes $ dest_RLPB nonce
+      ; value := num_of_be_bytes $ dest_RLPB value
+      ; gasLimit := num_of_be_bytes $ dest_RLPB gas
+      ; gasPrice := num_of_be_bytes $ dest_RLPB gasPrice
+      ; accessList := []
+      ; blobVersionedHashes := []
+      ; maxFeePerBlobGas := NONE
+      ; maxFeePerGas := NONE
+      |>
+  else let bs = dest_RLPB rlp in
+  if NULL bs then NONE else
+  if HD bs = 1w then
+    case rlp_decode (TL bs) of NONE => NONE |
+    SOME rlp => transaction1_from_rlp rlp
+  else if HD bs = 2w then
+    case rlp_decode (TL bs) of NONE => NONE |
+    SOME rlp => transaction2_from_rlp baseFee rlp
+  else if HD bs = 3w then
+    case rlp_decode (TL bs) of NONE => NONE |
+    SOME rlp => transaction3_from_rlp baseFee rlp
+  else NONE
+End
+
+val transaction_from_rlp_pre_def = cv_auto_trans_pre transaction_from_rlp_def;
+
+Theorem transaction_from_rlp_pre[cv_pre]:
+  transaction_from_rlp_pre bf x
+Proof
+  rw[transaction_from_rlp_pre_def]
+  \\ strip_tac \\ gvs[]
+QED
+
+Definition OPT_MMAP_transaction_from_rlp_def:
+  OPT_MMAP_transaction_from_rlp bf [] = SOME [] ∧
+  OPT_MMAP_transaction_from_rlp bf (x::xs) =
+  case transaction_from_rlp bf x of NONE => NONE
+     | SOME h =>
+         case OPT_MMAP_transaction_from_rlp bf xs of NONE => NONE
+            | SOME t => SOME (h::t)
+End
+
+val () = cv_auto_trans OPT_MMAP_transaction_from_rlp_def;
+
+Theorem OPT_MMAP_transaction_from_rlp_eq:
+  OPT_MMAP_transaction_from_rlp bf ls =
+  OPT_MMAP (transaction_from_rlp bf) ls
+Proof
+  Induct_on`ls` \\ rw[OPT_MMAP_transaction_from_rlp_def]
+  \\ CASE_TAC \\ gvs[]
+  \\ CASE_TAC \\ gvs[]
+QED
+
+Definition OPT_MMAP_withdrawal_from_rlp_def:
+  OPT_MMAP_withdrawal_from_rlp [] = SOME [] ∧
+  OPT_MMAP_withdrawal_from_rlp (x::xs) =
+  case withdrawal_from_rlp x of NONE => NONE
+     | SOME h =>
+         case OPT_MMAP_withdrawal_from_rlp xs of NONE => NONE
+            | SOME t => SOME (h::t)
+End
+
+val () = cv_auto_trans OPT_MMAP_withdrawal_from_rlp_def;
+
+Theorem OPT_MMAP_withdrawal_from_rlp_eq:
+  OPT_MMAP_withdrawal_from_rlp ls =
+  OPT_MMAP withdrawal_from_rlp ls
+Proof
+  Induct_on`ls` \\ rw[OPT_MMAP_withdrawal_from_rlp_def]
+  \\ CASE_TAC \\ gvs[]
+  \\ CASE_TAC \\ gvs[]
+QED
+
+Definition block_from_rlp_def:
+  block_from_rlp rlp =
+  if ¬is_RLPL rlp then NONE else
+  let ls = dest_RLPL rlp in
+  if LENGTH ls ≠ 4 then NONE else
+  let header = EL 0 ls in
+  let transactions = EL 1 ls in
+  let ommers = EL 2 ls in
+  let withdrawals = EL 3 ls in
+  case block_header_from_rlp header of NONE => NONE |
+  SOME blk =>
+  if ¬is_RLPL transactions then NONE else
+  let ls = dest_RLPL transactions in
+  case OPT_MMAP (transaction_from_rlp blk.baseFeePerGas) ls of NONE => NONE |
+  SOME transactions =>
+  if ¬is_RLPL withdrawals then NONE else
+  let ls = dest_RLPL withdrawals in
+  case OPT_MMAP withdrawal_from_rlp ls of NONE => NONE |
+  SOME withdrawals =>
+  SOME $
+    blk with <|
+      transactions := transactions
+    ; withdrawals := withdrawals
+    |>
+End
+
+val block_from_rlp_pre_def = block_from_rlp_def
+  |> SRULE [GSYM OPT_MMAP_withdrawal_from_rlp_eq,
+               GSYM OPT_MMAP_transaction_from_rlp_eq]
+  |> cv_auto_trans_pre;
+
+Theorem block_from_rlp_pre[cv_pre]:
+  block_from_rlp_pre x
+Proof
+  rw[block_from_rlp_pre_def]
+  \\ strip_tac \\ gvs[]
+QED
+
+(* -- *)
+
 Definition run_test_def:
   run_test fuel
     preState
-    (genesisRLP: byte list)
-    (genesisBlock: block)
+    genesisRLP
+    genesisBlock
     validBlocks
+    (validBlockRLPs: byte list list)
     lastBlockHash
     postState
     expectException
@@ -111,10 +502,10 @@ Definition run_test_def:
     case rlp_decode genesisRLP
     of NONE => GenesisBlockDecodeFailure |
     SOME rlp =>
-    case block_header_from_block_rlp rlp
+    case block_from_rlp rlp
     of NONE => GenesisBlockDecodeFailure |
-    SOME genesisHeader =>
-    if genesisHeader with hash := genesisBlock.hash <> genesisBlock
+    SOME decodedGenesisBlock =>
+    if decodedGenesisBlock with hash := genesisBlock.hash <> genesisBlock
     then GenesisBlockDecodeMismatch
     else case state_root_clocked fuel preState
     of NONE => OutOfFuel |
@@ -122,8 +513,9 @@ Definition run_test_def:
     let preStateRoot = word_of_bytes T 0w preStateRootBytes in
     if preStateRoot ≠ genesisBlock.stateRoot
     then GenesisHeaderMismatch preStateRoot
-    else case
-      (* TODO: check RLP decoding first *)
+    else
+      (* TODO: check validBlockRLPs decode to validBlocks *)
+    case
       run_blocks (Collect empty_domain) 1 [] genesisBlock preState validBlocks
     of NONE => UnexpectedException
      | SOME (_, hashes, parent, computedPostState, dom) =>
@@ -132,7 +524,7 @@ Definition run_test_def:
       if computedHash <> lastBlockHash then LastHashMismatch computedHash else
       if computedPostState <> postState then StateMismatch else Passed
     | SOME (msg, (rlp: word8 list), decoded) =>
-        (* TODO: check RLP *)
+        (* TODO: check rlp decodes to decoded *)
         case decoded of NONE => ExpectedException "block rlp decoding"
         | SOME invalidBlock =>
             case run_blocks dom 1 hashes parent computedPostState [invalidBlock] of
